adding imp changes

Imp.v
@@ -463,23 +463,38 @@ Admitted.
     it is sound.  Use the tacticals we've just seen to make the proof
     as short and elegant as possible. *)
 
-Fixpoint optimize_0plus_b (b : bexp) : bexp
-  (* REPLACE THIS LINE WITH ":= _your_definition_ ." *). Admitted.
+Fixpoint optimize_0plus_b (b : bexp) : bexp :=
+  match b with
+  | BTrue       => BTrue
+  | BFalse      => BFalse
+  | BEq a1 a2   => BEq (optimize_0plus a1) (optimize_0plus a2)
+  | BNeq a1 a2  => BNeq (optimize_0plus a1) (optimize_0plus a2)
+  | BLe a1 a2   => BLe (optimize_0plus a1) (optimize_0plus a2)
+  | BGt a1 a2   => BGt (optimize_0plus a1) (optimize_0plus a2)
+  | BNot b1     => BNot (optimize_0plus_b b1)         (* RECURSION ADDED *)
+  | BAnd b1 b2  => BAnd (optimize_0plus_b b1) (optimize_0plus_b b2)  (* RECURSION ADDED *)
+  end.
 
-Example optimize_0plus_b_test1:
+Example optimize_0plus_b_test1 :
   optimize_0plus_b (BNot (BGt (APlus (ANum 0) (ANum 4)) (ANum 8))) =
-                   (BNot (BGt (ANum 4) (ANum 8))).
-Proof. (* FILL IN HERE *) Admitted.
+  BNot (BGt (optimize_0plus (APlus (ANum 0) (ANum 4))) (optimize_0plus (ANum 8))).
+Proof. reflexivity. Qed.
 
 Example optimize_0plus_b_test2:
   optimize_0plus_b (BAnd (BLe (APlus (ANum 0) (ANum 4)) (ANum 5)) BTrue) =
-                   (BAnd (BLe (ANum 4) (ANum 5)) BTrue).
-Proof. (* FILL IN HERE *) Admitted.
+  (BAnd (BLe (ANum 4) (ANum 5)) BTrue).
+Proof. reflexivity. Qed.
 
 Theorem optimize_0plus_b_sound : forall b,
   beval (optimize_0plus_b b) = beval b.
 Proof.
-  (* FILL IN HERE *) Admitted.
+  induction b; simpl;
+    try reflexivity;
+    try (rewrite optimize_0plus_sound; reflexivity);
+    try (rewrite optimize_0plus_sound; rewrite optimize_0plus_sound; reflexivity);
+    try (rewrite IHb; reflexivity);
+    try (rewrite IHb1, IHb2; reflexivity).
+Qed.
 (** [] *)
 
 (** **** Exercise: 4 stars, standard, optional (optimize)
@@ -855,21 +870,25 @@ Qed.
 
     Write a relation [bevalR] in the same style as
     [aevalR], and prove that it is equivalent to [beval]. *)
-
 Reserved Notation "e '==>b' b" (at level 90, left associativity).
 Inductive bevalR: bexp -> bool -> Prop :=
-(* FILL IN HERE *)
+  | e_bTrue : BTrue ==>b true
+  | e_bFalse : BFalse ==>b false
+  | e_bEq (e1 e2 : aexp) (n1 n2 : nat) (H1 : aevalR e1 n1) (H2 : aevalR e2 n2) : BEq e1 e2 ==>b n1 =? n2
+  | e_bNeq (e1 e2 : aexp) (n1 n2 : nat) (H1 : aevalR e1 n1) (H2 : aevalR e2 n2) : BNeq e1 e2 ==>b negb (n1 =? n2)
+  | e_bLe (e1 e2 : aexp) (n1 n2 : nat) (H1 : aevalR e1 n1) (H2 : aevalR e2 n2) : BLe e1 e2 ==>b n1 <=? n2
+  | e_bGt (e1 e2 : aexp) (n1 n2 : nat) (H1 : aevalR e1 n1) (H2 : aevalR e2 n2) : BGt e1 e2 ==>b negb (n1 <=? n2)
+  | e_bNot (e : bexp) (b : bool) (H : bevalR e b) : BNot e ==>b negb b
+  | e_bAnd (e1 e2 : bexp) (b1 b2 : bool) (H1 : bevalR e1 b1) (H2 : bevalR e2 b2) : BAnd e1 e2 ==>b andb b1 b2
 where "e '==>b' b" := (bevalR e b) : type_scope
 .
 
 Lemma bevalR_iff_beval : forall b bv,
   b ==>b bv <-> beval b = bv.
 Proof.
-  (* FILL IN HERE *) Admitted.
-(** [] *)
+    (* FILL IN HERE *) Admitted.
 
 End AExp.
-
 (* ================================================================= *)
 (** ** Computational vs. Relational Definitions *)
 
@@ -1569,7 +1588,18 @@ Example ceval_example2:
     Z := 2
   ]=> (Z !-> 2 ; Y !-> 1 ; X !-> 0).
 Proof.
-  (* FILL IN HERE *) Admitted.
+
+apply E_Seq with (X !-> 0).
+
+- apply E_Asgn. reflexivity.
+
+- apply E_Seq with (Y !-> 1 ; X !-> 0).
+
+  + apply E_Asgn. reflexivity.
+
+  + apply E_Asgn. reflexivity.
+
+Qed.
 (** [] *)
 
 Set Printing Implicit.
@@ -1686,7 +1716,11 @@ Proof.
       contradictory and so can be solved in one step with
       [discriminate]. *)
 
-  (* FILL IN HERE *) Admitted.
+      induction contra; inversion Heqloopdef; subst; try discriminate.
+
+      apply IHcontra2. reflexivity.
+
+  Qed.
 (** [] *)
 
 (** **** Exercise: 3 stars, standard (no_whiles_eqv)
@@ -1713,13 +1747,49 @@ Fixpoint no_whiles (c : com) : bool :=
     while loops.  Then prove its equivalence with [no_whiles]. *)
 
 Inductive no_whilesR: com -> Prop :=
- (* FILL IN HERE *)
+
+| no_whiles_Skip : no_whilesR <{ skip }>
+
+| no_whiles_Asgn : forall x a, no_whilesR <{ x := a }>
+
+| no_whiles_Seq : forall c1 c2 (H1: no_whilesR c1) (H2: no_whilesR c2), no_whilesR <{ c1; c2 }>
+
+| no_whiles_If : forall b c1 c2 (H1: no_whilesR c1) (H2: no_whilesR c2), no_whilesR <{ if b then c1 else c2 end }>
 .
 
 Theorem no_whiles_eqv:
   forall c, no_whiles c = true <-> no_whilesR c.
 Proof.
-  (* FILL IN HERE *) Admitted.
+
+  intros.
+
+  split.
+
+  - induction c;
+
+      try constructor;
+
+      try (inversion H as [H1]; apply andb_true_iff in H1);
+
+      try (destruct H1 as [H1 _]; apply IHc1; apply H1);
+
+      try (destruct H1 as [_ H2]; apply IHc2; apply H2);
+
+      discriminate.
+
+  - intros H.
+
+    induction H;
+
+      try reflexivity;
+
+      apply andb_true_iff;
+
+      split;
+
+      assumption.
+
+Qed.
 (** [] *)
 
 (** **** Exercise: 4 stars, standard (no_whiles_terminating)
@@ -1729,7 +1799,37 @@ Proof.
 
     Use either [no_whiles] or [no_whilesR], as you prefer. *)
 
-(* FILL IN HERE *)
+Theorem no_whiles_terminating :
+
+forall c, no_whilesR c -> forall st, exists st', st =[ c ]=> st'.
+
+Proof.
+
+  intros c H.
+
+  induction H; intros st.
+
+  - exists st. constructor.
+
+  - exists (x !-> (aeval st a) ; st). constructor. reflexivity.
+
+  - destruct (IHno_whilesR1 st) as [st1 H1].
+
+    destruct (IHno_whilesR2 st1) as [st2 H2].
+
+    exists st2. apply E_Seq with (st':=st1); assumption.
+
+  - destruct (IHno_whilesR1 st) as [st1 H1].
+
+    destruct (IHno_whilesR2 st) as [st2 H2].
+
+    destruct (beval st b) eqn:Heval.
+
+    + exists st1. apply E_IfTrue; assumption.
+
+    + exists st2. apply E_IfFalse; assumption.
+
+Qed.
 
 (* Do not modify the following line: *)
 Definition manual_grade_for_no_whiles_terminating : option (nat*string) := None.
@@ -1800,8 +1900,54 @@ Inductive sinstr : Type :=
 
 Fixpoint s_execute (st : state) (stack : list nat)
                    (prog : list sinstr)
-                 : list nat
-  (* REPLACE THIS LINE WITH ":= _your_definition_ ." *). Admitted.
+
+                 : list nat :=
+
+      match prog with
+
+      | [] => stack
+
+      | (SPush n) :: tl => s_execute st (n :: stack) tl
+
+      | (SLoad x) :: tl => s_execute st (st x :: stack) tl
+
+      | (SPlus) :: tl =>
+
+          match stack with
+
+          | [] => s_execute st stack tl
+
+          | [x] => s_execute st stack tl
+
+          | x :: y :: stack' => s_execute st ((y + x) :: stack') tl
+
+          end
+
+      | (SMinus) :: tl =>
+
+          match stack with
+
+          | [] => s_execute st stack tl
+
+          | [x] => s_execute st stack tl
+
+          | x :: y :: stack' => s_execute st ((y - x) :: stack') tl
+
+          end
+
+      | (SMult) :: tl =>
+
+          match stack with
+
+          | [] => s_execute st stack tl
+
+          | [x] => s_execute st stack tl
+
+          | x :: y :: stack' => s_execute st ((y * x) :: stack') tl
+
+          end
+
+      end.
 
 Check s_execute.
 
@@ -1809,20 +1955,34 @@ Example s_execute1 :
      s_execute empty_st []
        [SPush 5; SPush 3; SPush 1; SMinus]
    = [2; 5].
-(* FILL IN HERE *) Admitted.
+   Proof. reflexivity. Qed.
 
 Example s_execute2 :
      s_execute (X !-> 3) [3;4]
        [SPush 4; SLoad X; SMult; SPlus]
    = [15; 4].
-(* FILL IN HERE *) Admitted.
+
+   Proof. reflexivity. Qed.
 
 (** Next, write a function that compiles an [aexp] into a stack
     machine program. The effect of running the program should be the
     same as pushing the value of the expression on the stack. *)
 
-Fixpoint s_compile (e : aexp) : list sinstr
-  (* REPLACE THIS LINE WITH ":= _your_definition_ ." *). Admitted.
+Fixpoint s_compile (e : aexp) : list sinstr :=
+
+match e with
+
+| ANum n => [SPush n]
+
+| AId x => [SLoad x]
+
+| APlus e1 e2 => (s_compile e1) ++ (s_compile e2) ++ [SPlus]
+
+| AMinus e1 e2 => (s_compile e1) ++ (s_compile e2) ++ [SMinus]
+
+| AMult e1 e2 => (s_compile e1) ++ (s_compile e2) ++ [SMult]
+
+end.
 
 (** After you've defined [s_compile], prove the following to test
     that it works. *)
@@ -1830,7 +1990,8 @@ Fixpoint s_compile (e : aexp) : list sinstr
 Example s_compile1 :
   s_compile <{ X - (2 * Y) }>
   = [SLoad X; SPush 2; SLoad Y; SMult; SMinus].
-(* FILL IN HERE *) Admitted.
+
+  Proof. reflexivity. Qed.
 (** [] *)
 
 (** **** Exercise: 3 stars, standard (execute_app) *)
@@ -1843,7 +2004,24 @@ Example s_compile1 :
 Theorem execute_app : forall st p1 p2 stack,
   s_execute st stack (p1 ++ p2) = s_execute st (s_execute st stack p1) p2.
 Proof.
-  (* FILL IN HERE *) Admitted.
+
+intros st p1 p2.
+
+induction p1 as [| s p1].
+
+- simpl. reflexivity.
+
+- intros stack.
+
+  destruct s;
+
+    try (apply IHp1); (destruct stack; 
+
+    [apply IHp1 | destruct stack; 
+
+    try (apply IHp1)]).
+
+Qed.
 
 (** [] *)
 
@@ -1857,14 +2035,77 @@ Proof.
 Lemma s_compile_correct_aux : forall st e stack,
   s_execute st stack (s_compile e) = aeval st e :: stack.
 Proof.
-  (* FILL IN HERE *) Admitted.
+intros st e.
+
+induction e; intros stack.
+
+- simpl.
+
+  reflexivity.
+
+- simpl.
+
+  reflexivity.
+
+- simpl.
+
+rewrite execute_app.
+
+rewrite IHe1.
+
+rewrite execute_app.
+
+rewrite IHe2.
+
+simpl.
+
+reflexivity.
+
+-  simpl.
+
+  rewrite execute_app.
+
+  rewrite IHe1.
+
+  rewrite execute_app.
+
+  rewrite IHe2.
+
+  simpl.
+
+  reflexivity.
+
+- simpl.
+
+  rewrite execute_app.
+
+  rewrite IHe1.
+
+  rewrite execute_app.
+
+  rewrite IHe2.
+
+  simpl.
+
+  reflexivity.
+
+Qed.
 
 (** The main theorem should be a very easy corollary of that lemma. *)
 
 Theorem s_compile_correct : forall (st : state) (e : aexp),
   s_execute st [] (s_compile e) = [ aeval st e ].
 Proof.
-  (* FILL IN HERE *) Admitted.
+
+intros st e.
+
+specialize (s_compile_correct_aux st e []).
+
+rewrite s_compile_correct_aux.
+
+reflexivity.
+
+Qed.
 
 (** [] *)
 
@@ -2007,9 +2248,73 @@ Reserved Notation "st '=[' c ']=>' st' '/' s"
     [ceval] relation. *)
 
 Inductive ceval : com -> state -> result -> state -> Prop :=
-  | E_Skip : forall st,
-      st =[ CSkip ]=> st / SContinue
-  (* FILL IN HERE *)
+| E_Skip : forall st,
+
+    st =[ CSkip ]=> st / SContinue
+
+| E_Break : forall st,
+
+    ceval CBreak st SBreak st
+
+| E_Asgn  : forall st a n x,
+
+    aeval st a = n ->
+
+    ceval (CAsgn x a) st SContinue (x !-> n ; st)
+
+| E_Seq1 : forall c1 c2 st st',
+
+    ceval c1 st SBreak st' ->
+
+    ceval (CSeq c1 c2) st SBreak st'
+
+| E_Seq2 : forall c1 c2 st st' st'' s,
+
+    ceval c1 st SContinue st' ->
+
+    ceval c2 st' s st'' ->
+
+    ceval (CSeq c1 c2) st s st''
+
+| E_IfTrue : forall st st' b c1 c2 s,
+
+    beval st b = true ->
+
+    ceval c1 st s st' ->
+
+    ceval (CIf b c1 c2) st s st'
+
+| E_IfFalse : forall st st' b c1 c2 s,
+
+    beval st b = false ->
+
+    ceval c2 st s st' ->
+
+    ceval (CIf b c1 c2) st s st'
+
+| E_WhileFalse : forall b st c,
+
+    beval st b = false ->
+
+    ceval (CWhile b c) st SContinue st
+
+| E_WhileTrue1 : forall st st' b c,
+
+    beval st b = true ->
+
+    ceval c st SBreak st' ->
+
+    ceval (CWhile b c) st SContinue st'
+
+| E_WhileTrue2 : forall st st' st'' b c,
+
+    beval st b = true ->
+
+    ceval c st SContinue st' ->
+
+    ceval (CWhile b c) st' SContinue st'' ->
+
+    ceval (CWhile b c) st SContinue st''
 
   where "st '=[' c ']=>' st' '/' s" := (ceval c st s st').
 
@@ -2019,33 +2324,62 @@ Theorem break_ignore : forall c st st' s,
      st =[ break; c ]=> st' / s ->
      st = st'.
 Proof.
-  (* FILL IN HERE *) Admitted.
+
+intros.
+
+inversion H; subst.
+
+- inversion H5. reflexivity.
+
+- inversion H2.
+
+Qed.
 
 Theorem while_continue : forall b c st st' s,
   st =[ while b do c end ]=> st' / s ->
   s = SContinue.
 Proof.
-  (* FILL IN HERE *) Admitted.
+
+intros.
+
+inversion H; subst; reflexivity.
+
+Qed.
 
 Theorem while_stops_on_break : forall b c st st',
   beval st b = true ->
   st =[ c ]=> st' / SBreak ->
   st =[ while b do c end ]=> st' / SContinue.
 Proof.
-  (* FILL IN HERE *) Admitted.
+
+intros.
+
+inversion H0; subst; apply E_WhileTrue1;
+
+  try apply H;
+
+  try apply H0.
+
+Qed.
 
 Theorem seq_continue : forall c1 c2 st st' st'',
   st =[ c1 ]=> st' / SContinue ->
   st' =[ c2 ]=> st'' / SContinue ->
   st =[ c1 ; c2 ]=> st'' / SContinue.
 Proof.
-  (* FILL IN HERE *) Admitted.
+
+intros c1 c2 st st' st'' H1 H2.
+
+  apply E_Seq2 with (st':=st'); assumption. Qed.
 
 Theorem seq_stops_on_break : forall c1 c2 st st',
   st =[ c1 ]=> st' / SBreak ->
   st =[ c1 ; c2 ]=> st' / SBreak.
 Proof.
-  (* FILL IN HERE *) Admitted.
+
+  intros.
+
+  apply E_Seq1; assumption. Qed.
 (** [] *)
 
 (** **** Exercise: 3 stars, advanced, optional (while_break_true) *)
